translator/lean/corellzk2smt/Corellzk2smt/SymExec/ArrayCmds.lean
@@ -1,0 +1,64 @@
+import Corellzk2smt.Basic
+import Corellzk2smt.Config
+import Corellzk2smt.SymExec.Basic
+import Corellzk2smt.SymExec.Common
+import Corellzk2smt.FFConstraints.Basic
+import Corellzk2smt.Language.Core.Syntax.AST
+
+
+namespace Corellzk2smt.SymExec.BigStep
+
+
+open Corellzk2smt.Config (GlobalConfig)
+open Corellzk2smt.Language.Core.Syntax.AST
+open Corellzk2smt.SymExec.Basic
+open Corellzk2smt.FFConstraints.Basic
+
+
+def seNewArray {c : ZKConfig}
+    (_md : CmdMD)
+    (_gconf : GlobalConfig c)
+    (_sconf : SymExecConfig c)
+    (_symEnv : SymEnv c)
+    (_specs : List (FuncSpec c))
+    (_id : VarID)
+    (_size : SimpleExpr c)
+    : Except String (CmdsSpec c) :=
+  Except.error "seNewArray: TBD"
+
+def seReadArray {c : ZKConfig}
+    (_md : CmdMD)
+    (_gconf : GlobalConfig c)
+    (_sconf : SymExecConfig c)
+    (_symEnv : SymEnv c)
+    (_specs : List (FuncSpec c))
+    (_out : VarID)
+    (_a : VarID)
+    (_index : SimpleExpr c)
+    : Except String (CmdsSpec c) :=
+  Except.error "seReadArray: TBD"
+
+def seWriteArray {c : ZKConfig}
+    (_md : CmdMD)
+    (_gconf : GlobalConfig c)
+    (_sconf : SymExecConfig c)
+    (_symEnv : SymEnv c)
+    (_specs : List (FuncSpec c))
+    (_a : VarID)
+    (_index : SimpleExpr c)
+    (_value : SimpleExpr c)
+    : Except String (CmdsSpec c) :=
+  Except.error "seWriteArray: TBD"
+
+def seCopyArray {c : ZKConfig}
+    (_md : CmdMD)
+    (_gconf : GlobalConfig c)
+    (_sconf : SymExecConfig c)
+    (_symEnv : SymEnv c)
+    (_specs : List (FuncSpec c))
+    (_out : VarID)
+    (_a : VarID)
+    : Except String (CmdsSpec c) :=
+  Except.error "seCopyArray: TBD"
+
+end Corellzk2smt.SymExec.BigStep
