translator/lean/corellzk2smt/Corellzk2smt/SymExec/Assignment.lean
@@ -1,0 +1,28 @@
+import Corellzk2smt.Basic
+import Corellzk2smt.Config
+import Corellzk2smt.SymExec.Basic
+import Corellzk2smt.SymExec.Common
+import Corellzk2smt.FFConstraints.Basic
+import Corellzk2smt.Language.Core.Syntax.AST
+
+
+namespace Corellzk2smt.SymExec.BigStep
+
+
+open Corellzk2smt.Config (GlobalConfig)
+open Corellzk2smt.Language.Core.Syntax.AST
+open Corellzk2smt.SymExec.Basic
+open Corellzk2smt.FFConstraints.Basic
+
+def seEvalAssignment {c : ZKConfig}
+    (_md : CmdMD)
+    (_gconf : GlobalConfig c)
+    (_sconf : SymExecConfig c)
+    (_symEnv : SymEnv c)
+    (_specs : List (FuncSpec c))
+    (_id : VarID)
+    (_e : Expr c)
+    : Except String (CmdsSpec c) :=
+  Except.error "seEvalAssign: TBD"
+
+end Corellzk2smt.SymExec.BigStep
